cfrontend/CexecExprProof.v
@@ -1,0 +1,1639 @@
+Require Import FunInd.
+Require Import FunctionalExtensionality.
+Require Import Axioms Classical.
+Require Import String Coqlib Decidableplus.
+Require Import Errors Maps Integers Floats.
+Require Import AST Values Memory AllocatorImpl Allocator Events Globalenvs Builtins Csem.
+Require Import Tags.
+Require Import List. Import ListNotations.
+Require Import Cexec Ctypes.
+Require Import ExtLib.Structures.Monads. Import MonadNotation.
+
+Local Open Scope list_scope.
+
+Module ExprProof (Pol: Policy).
+  Module Cexec := Cexec Pol.
+  Module Inner (I: AllocatorImpl ConcretePointer Pol Cexec.CM).
+    Module CexecInner := Cexec.Inner I.
+    Import CexecInner.
+    Import A.
+    Import ConcretePointer.
+
+    Local Open Scope option_monad_scope.
+
+    Ltac doinv :=
+      match goal with
+      | [ H: _ <- ?e ;; _ = Some _ |- _ ] => destruct e eqn:?; [simpl in H| inv H]
+      | [ H: let _ := ?e in _ |- _ ] => destruct e eqn:?
+      | [ H: is_val ?e = _ |- context[?e] ] => rewrite (is_val_inv _ _ _ H)
+      | [ H1: is_val ?e = _, H2: context[?e] |- _ ] => rewrite (is_val_inv _ _ _ H1) in H2
+      | [ H: is_loc ?e = _ |- context[?e] ] => rewrite (is_loc_inv _ _ _ H)
+      | [ H1: is_loc ?e = _, H2: context[?e] |- _ ] => rewrite (is_loc_inv _ _ _ H1) in H2
+      | [ p : _ * _ |- _ ] => destruct p
+      | [ a: atom |- _ ] => destruct a eqn:?; subst a
+      | [ H: False |- _ ] => destruct H
+      | [ H: _ /\ _ |- _ ] => destruct H
+      | [ H: _ \/ _ |- _ ] => destruct H
+      | [ H: exists _, _ |- _ ] => destruct H
+      | [H: bind_prop_success_rel ?e _ _ _ |- _ ] =>
+          let res := fresh "res" in
+          let H' := fresh "H" in
+          let RES := fresh "RES" in
+          inversion H as [res [H' RES]]; clear H
+      | [ H: Vptr _ = Vnullptr |- _ ] => inv H
+      | [H: is_ptr ?v = Some _ |- _] => destruct v; simpl in H; try discriminate
+      | [ H: Int64.eq _ _ = true |- _ ] => apply Int64.same_if_eq in H
+      | [ H: Int64.eq ?v1 ?v2 = false |- _] =>
+          assert (v1 <> v2) by (intro; subst; rewrite (Int64.eq_true v2) in H; discriminate);
+          clear H
+      | [ H: (_,_) = (_,_) |- _ ] => inv H
+      | [ H: (_,_,_) = (_,_,_) |- _ ] => inv H
+      | [ H: possible_trace ?w (?tr1 ++ ?tr2) ?w' |- _ ] =>
+          let w := fresh "w" in
+          let H1 := fresh "H" in
+          let H2 := fresh "H" in
+          eapply possible_trace_app_inv in H;
+          destruct H as [w [H1 H2]]
+      | [ H: possible_trace ?w E0 ?w' |- _ ] => inv H
+      | _ => idtac
+      end.
+
+    Ltac dodestr :=
+      match goal with
+      | [ |- context [match ?e with
+                      | Some _ => _
+                      | _ => _
+                      end] ] =>
+          destruct e eqn:?
+      | [ |- context [check ?e ; _] ] =>
+          destruct e eqn:?
+      | [ |- context [match ?e with
+                      | Success _ => _
+                      | Fail _ => _
+                      end] ] =>
+          destruct e eqn:?
+      | [ |- context [match ?e with
+                      | inl _ => _
+                      | inr _ => _
+                      end] ] =>
+          destruct e eqn:?
+      | [ |- context [match ?e with
+                      | PRIV _ => _
+                      | PUB _ _ _ => _
+                      end] ] =>
+          destruct e eqn:?
+      | [ |- context [match ?ty with
+                      | Tstruct _ _ => _
+                      | _ => _
+                      end] ] =>
+          destruct ty eqn:?
+      | [ |- context [match ?e with
+                      | OK _ => _
+                      | Error _ => _
+                      end] ] =>
+          destruct e eqn:?
+      | [ |- context [if ?e then _ else _] ] => destruct e eqn:?
+      | [ |- context [match ?v with
+                      | Vptr _ => _
+                      | _ => _
+                      end] ] => destruct v
+      | [ |- context [match ?l with
+                      | Lmem _ _ _ => _
+                      | Ltmp _ => _
+                      | Lifun _ _ => _
+                      | Lefun _ _ _ _ _ => _
+                      end] ] => destruct l
+      | [ |- context [match ?e with
+                      | fun_case_f _ _ _ => _
+                      | fun_default => _
+                      end] ] => destruct e eqn:?
+      | [ |- context [let '(_, _) := ?e in _] ] =>
+          destruct e eqn:?
+      | [ |- context [sem_unary_operation ?op ?v ?ty ?m] ] =>
+          destruct (sem_unary_operation op v ty m) eqn:?
+      | [ |- context [sem_binary_operation ?ce ?op ?v ?ty1 ?v2 ?ty2 ?m] ] =>
+          destruct (sem_binary_operation ce op v ty1 v2 ty2 m) eqn:?
+      | [ |- context [sem_cast ?v ?ty1 ?ty2 ?m] ] =>
+          destruct (sem_cast v ty1 ty2 m) eqn:?
+      | [ |- context [bool_val ?v ?ty ?m] ] =>
+          destruct (bool_val v ty m) eqn:?
+      | _ => idtac
+      end.
+
+      Ltac cronch :=
+        match goal with
+        | [ H: ?e1 = None
+            |- context[?e1]] => rewrite H
+        | [ H: ?e1 = Some _
+            |- context[?e1]] => rewrite H
+        | [ H: ?e ! ?b = Some _ |- context [?e ! ?b]] => rewrite H
+        | [ H: ?e ! ?b = None |- context [?e ! ?b]] => rewrite H
+        | [ H: ?e1 = (Success _, _) |- context[?e1] ] =>
+            rewrite H; simpl
+        | [ H: ?e1 = (Fail _, _) |- context[?e1] ] =>
+            rewrite H; simpl
+        | [ H: ?e = true |- (if ?e then _ else _) = _ ] => rewrite H
+        | [ H: ?e = false |- (if ?e then _ else _) = _ ] => rewrite H
+        | [ H: ?v = Vptr ?v' |- match ?v with
+                                | Vptr _ => _
+                                | _ => _
+                                end = _ ] =>
+            rewrite H
+        | [ H: access_mode ?ty = ?e |- context [match access_mode ?ty with
+                                                | By_value _ => _
+                                                | _ => _
+                                                end ]] =>
+            rewrite H
+        | [ |- context [type_eq ?ty ?ty] ] => rewrite dec_eq_true
+        | [ H: possible_trace ?w ?tr ?w' |- possible_trace ?w ?tr _ ] => apply H
+        | [ |- exists w' : world, possible_trace ?w E0 w' ] =>
+            exists w; constructor
+        | [ H: ?e ?ps |- bind_prop_success_rel ?e _ _ _ ] =>
+            exists ps; intuition eauto
+        end.
+    
+    Section EXEC.
+      Variable ge: genv.
+      Variable ce: composite_env.
+    
+      Variable do_external_function:
+        Cabs.loc -> string -> signature -> Genv.t fundef type -> world -> list atom ->
+        control_tag -> val_tag -> mem ->
+        option (world * trace * (PolicyResult (atom * control_tag * mem))).
+
+      Hypothesis do_external_function_sound:
+        forall lc id sg ge vargs pct fpt m t res w w',
+          do_external_function lc id sg ge w vargs pct fpt m = Some(w', t, res) ->
+          external_functions_sem lc id sg tt ge vargs pct fpt m t res /\ possible_trace w t w'.
+    
+      Hypothesis do_external_function_complete:
+        forall lc id sg ge vargs pct fpt m t res w w',
+          external_functions_sem lc id sg tt ge vargs pct fpt m t res ->
+          possible_trace w t w' ->
+          do_external_function lc id sg ge w vargs pct fpt m = Some(w', t, res).
+
+      Lemma do_deref_loc_sound:
+        forall w ty m ofs pt bf w' t res,
+          do_deref_loc ge w ty m ofs pt bf = Some (w', t, res) ->
+          deref_loc ge ty m ofs pt bf t res /\ possible_trace w t w'.
+      Proof.
+        unfold do_deref_loc; intros until res.
+        destruct bf.
+        - destruct (access_mode ty) eqn:?; mydestr; try congruence.
+          + intros. exploit do_volatile_load_sound; eauto.
+            intuition. eapply deref_loc_volatile; eauto.
+          + intros. split.
+            * eapply deref_loc_value; eauto.
+            * constructor.
+          + split. inv Heqm0.
+            eapply deref_loc_reference; eauto. inv Heqm0. constructor.
+          + split. inv Heqm0. eapply deref_loc_copy; eauto. inv Heqm0. constructor.
+        - destruct ty; try congruence.
+          dodestr; try congruence.
+          intros. InvBooleans. subst i.
+          inv H.
+          split; constructor.
+          econstructor; eauto.
+      Qed.
+    
+      Lemma do_deref_loc_complete:
+        forall w ty m ofs pt bf w' t res,
+          deref_loc ge ty m ofs pt bf t res -> possible_trace w t w' ->
+          do_deref_loc ge w ty m ofs pt bf = Some (w', t, res).
+      Proof.
+        unfold do_deref_loc; intros. inv H.
+        - rewrite H1.
+          inv H0. rewrite H2. auto.
+        - repeat cronch. apply (do_volatile_load_complete ge w _ _ _ w') in H3; auto.
+        - inv H0. rewrite H1. auto.
+        - inv H0. rewrite H1. auto.
+        - inv H0. inv H1.
+          unfold proj_sumbool; rewrite ! dec_eq_true, ! zle_true, ! zlt_true by lia. cbn. auto.
+      Qed.
+
+      Lemma do_assign_loc_sound:
+        forall w ty m ofs pt bf v vt w' t lts res,
+          do_assign_loc ge ce w ty m ofs pt bf (v,vt) lts = Some (w', t, res) ->
+          assign_loc ge ce ty m ofs pt lts bf (v,vt) t res /\ possible_trace w t w'.
+      Proof.
+        Local Opaque ret.
+        unfold do_assign_loc; intros until res.
+        destruct bf.
+        - destruct (access_mode ty) eqn:?; mydestr; try congruence.
+          + intros. repeat doinv. inv H.
+            exploit do_volatile_store_sound; eauto.
+            intros (P & Q). intuition. eapply assign_loc_volatile; eauto.
+          + split; econstructor; eauto.
+          + destruct v; mydestr; try congruence.
+            destruct a as [P [Q R]].
+            split.
+            apply assign_loc_copy; auto.
+            constructor.
+        - repeat dodestr; intros; InvBooleans; destruct ty; try congruence; subst.
+          + inv H. split. eapply assign_loc_bitfield; eauto.
+            econstructor; eauto. constructor.
+      Qed.
+    
+    Lemma do_assign_loc_complete:
+      forall w ty m ofs pt bf v vt w' t res lts,
+        assign_loc ge ce ty m ofs pt lts bf (v,vt) t res -> possible_trace w t w' ->
+        do_assign_loc ge ce w ty m ofs pt bf (v,vt) lts = Some (w', t, res).
+    Proof.
+      unfold do_assign_loc; intros. inv H; repeat cronch; auto.
+      - inv H0; auto.
+      - eapply do_volatile_store_complete in H3; eauto.
+        rewrite H3. auto.
+      - inv H0. repeat dodestr; auto.
+        elim n. red; tauto.
+      - inv H0. inv H1.
+        + unfold proj_sumbool; rewrite ! zle_true, ! zlt_true by lia.
+          rewrite ! dec_eq_true. cbn. repeat cronch. auto.
+    Qed.
+
+    Lemma is_val_list_preserves_len :
+      forall rargs vtl,
+        is_val_list rargs = Some vtl ->
+        exprlist_len rargs = List.length vtl.
+    Proof.
+      induction rargs.
+      - intros. inv H. auto.
+      - intros. inv H. destruct (is_val r1); try discriminate.
+        destruct (is_val_list rargs); try discriminate.
+        inv H1. simpl. specialize IHrargs with l. rewrite IHrargs; auto.
+    Qed.
+    
+    Lemma sem_cast_arguments_sound:
+      forall lc pct fpt rargs vtl tyargs res r ps ps',
+        is_val_list rargs = Some vtl ->
+        sem_cast_arguments lc pct fpt vtl tyargs = Some res ->
+        res ps = (r, ps') ->
+        cast_arguments lc pct ps fpt tt rargs tyargs ps' r.
+    Proof.
+      intros until rargs. generalize dependent pct.
+      induction rargs; simpl; intros.
+      - inv H. destruct tyargs; simpl in H0; inv H0. inv H1. constructor. 
+      - destruct (is_val r1) eqn:?; try discriminate.
+        destruct (is_val_list rargs) eqn:?; try discriminate.
+        inv H. simpl in H0. destruct p as [[v1 t1] ty1].
+        rewrite <- (is_val_list_preserves_len _ _ Heqo0) in *; eauto.
+        rewrite (is_val_inv _ _ _ Heqo). 
+        destruct tyargs; try congruence.
+        destruct (sem_cast_arguments lc pct fpt l tyargs) eqn:?; try discriminate.
+        destruct (sem_cast v1 ty1 t0 tt) eqn:?; try discriminate.
+        inv H0.
+        unfold bind_res in H1. destruct (p ps) eqn:?. destruct r0.
+        + destruct res. destruct (ArgT lc c fpt t1 (exprlist_len rargs) t0 p0) as
+            [[[pct' vt']|failure] p1] eqn:?.
+          * inv H1. econstructor; eauto.
+          * inv H1. econstructor; eauto.
+        + inv H1. eapply cast_args_fail_later; eauto.
+    Qed.
+    
+    Lemma sem_cast_arguments_complete:
+      forall al tyl r lc pct ps fpt ps',
+        cast_arguments lc pct ps fpt tt al tyl ps' r ->
+        exists vtl res, is_val_list al = Some vtl /\
+                          sem_cast_arguments lc pct fpt vtl tyl = Some res /\
+                          res ps = (r, ps').
+    Proof.
+      induction 1.
+      - exists (@nil (atom * type)), (fun ps => (Success (pct, @nil atom), ps)); auto.
+      - destruct IHcast_arguments as [vtl [res [A [B C]]]].
+        exists (((v,vt), ty) :: vtl).
+        eexists. simpl. rewrite A. split; auto.
+        rewrite B. rewrite H0. split; [reflexivity|].
+        unfold bind_res. rewrite C. rewrite <- (is_val_list_preserves_len _ _ A).
+        rewrite H1. auto.
+      - destruct IHcast_arguments as [vtl [res [A [B C]]]].
+        exists (((v,vt), ty) :: vtl).
+        eexists. simpl. rewrite A. split; auto.
+        rewrite B. rewrite H0. split; [reflexivity|].
+        unfold bind_res. rewrite C. rewrite <- (is_val_list_preserves_len _ _ A).
+        rewrite H1. auto.
+      - destruct IHcast_arguments as [vtl [res [A [B C]]]].
+        exists (((v,vt), ty) :: vtl).
+        eexists. simpl. rewrite A. split; auto.
+        rewrite B. rewrite H0. split; [reflexivity|].
+        unfold bind_res. rewrite C. auto.
+    Qed.
+        
+    Section EXPRS.
+      
+      Variable e: env.
+      Variable w: world.
+
+      Definition invert_expr_prop (lc:Cabs.loc) (a: expr) (ps: pstate) (pct: control_tag) (te: tenv)
+                 (m: mem) : Prop :=
+        match a with
+        | Eloc l ty => False
+        | Evar x ty =>
+            e!x = Some (PRIV ty)
+            \/ (exists base pt, e!x = Some (PUB base pt ty))
+            \/ (e!x = None /\ exists base bound pt gv,
+                   Genv.find_symbol ge x = Some (SymGlob base bound pt gv))
+            \/ (e!x = None /\ exists b pt, Genv.find_symbol ge x = Some (SymIFun _ b pt))
+            \/ (e!x = None /\ exists ef tyargs tyres cc pt,
+                   Genv.find_symbol ge x = Some (SymEFun _ ef tyargs tyres cc pt))
+        | Ederef (Eval (v,pt) ty1) ty =>
+            exists p,
+            sem_cast v ty1 ty1 tt = Some (Vptr p)
+        | Eaddrof (Eloc (Lmem ofs pt bf) ty1) ty =>
+            bf = Full
+        | Eaddrof (Eloc (Ltmp b) ty1) ty =>
+            False
+        | Eaddrof (Eloc (Lifun b pt) ty1) ty =>
+            ty = ty1
+        | Eaddrof (Eloc (Lefun _ _ _ _ pt) ty1) ty =>
+            ty = ty1
+        | Efield (Eval (v,vt) ty1) f ty =>
+            exists p, v = Vptr p /\
+                        match ty1 with
+                        | Tstruct id _ => exists co delta bf,
+                            ce!id = Some co /\
+                              field_offset ce f (co_members co) = OK (delta, bf)
+                        | Tunion id _ => exists co delta bf,
+                            ce!id = Some co /\
+                              union_field_offset ce f (co_members co) = OK (delta, bf)
+                        | _ => False
+                        end
+        | Eval v ty => False
+        | Evalof (Eloc (Lmem ofs pt bf) ty1) ty
+        | Eassignop _ (Eloc (Lmem ofs pt bf) ty1) (Eval _ _) _ ty
+        | Epostincr _ (Eloc (Lmem ofs pt bf) ty1) ty =>
+            exists t res w',
+            ty = ty1 /\ deref_loc ge ty1 m ofs pt bf t res /\ possible_trace w t w'
+        | Evalof (Eloc (Ltmp b) ty1) ty
+        | Eassignop _ (Eloc (Ltmp b) ty1) (Eval _ _) _ ty
+        | Epostincr _ (Eloc (Ltmp b) ty1) ty =>
+            exists v vt, ty = ty1 /\ te!b = Some (v,vt)
+        | Evalof (Eloc (Lifun _ _) ty1) ty
+        | Evalof (Eloc (Lefun _ _ _ _ _) ty1) ty
+        | Eassignop _ (Eloc (Lifun _ _) ty1) (Eval _ _) _ ty
+        | Eassignop _ (Eloc (Lefun _ _ _ _ _) ty1) (Eval _ _) _ ty
+        | Epostincr _ (Eloc (Lifun _ _) ty1) ty =>
+            ty = ty1
+        | Epostincr _ (Eloc (Lefun _ _ _ _ _) ty1) ty =>
+            ty = ty1
+        | Eunop op (Eval (v1,vt1) ty1) ty =>
+            exists v, sem_unary_operation op v1 ty1 m = Some v
+        | Ebinop op (Eval (v1,vt1) ty1) (Eval (v2,vt2) ty2) ty =>
+            exists v, sem_binary_operation ce op v1 ty1 v2 ty2 tt = Some v
+        | Ecast (Eval (v1,vt1) (Tpointer ty1 attr1)) (Tpointer ty attr) =>
+            exists p,
+            sem_cast v1 (Tpointer ty1 attr1) (Tpointer ty attr) tt = Some (Vptr p) /\
+              (~ Vnullptr (Vptr p) ->
+               exists tr w' res v2 vt2 lts ps',
+                 deref_loc ge (Tpointer ty attr) m p vt1 Full tr res /\
+                   res ps = (Success ((v2,vt2), lts), ps') /\
+                   possible_trace w tr w')
+        | Ecast (Eval (v1,vt1) ty1) (Tpointer ty attr) =>
+            exists p,
+            sem_cast v1 ty1 (Tpointer ty attr) tt = Some (Vptr p) /\
+              (~ Vnullptr (Vptr p) ->
+               exists tr w' res v2 vt2 lts ps',
+                 deref_loc ge (Tpointer ty attr) m p vt1 Full tr res /\
+                   res ps = (Success ((v2,vt2), lts), ps') /\
+                   possible_trace w tr w')
+        | Ecast (Eval (v1,vt1) ty1) ty =>
+            exists v, sem_cast v1 ty1 ty tt = Some v
+        | Eseqand (Eval (v1,vt1) ty1) r2 ty =>
+            exists b, bool_val v1 ty1 m = Some b
+        | Eseqor (Eval (v1,vt1) ty1) r2 ty =>
+            exists b, bool_val v1 ty1 m = Some b
+        | Econdition (Eval (v1,vt1) ty1) r1 r2 ty =>
+            exists b, bool_val v1 ty1 m = Some b
+        | Eassign (Eloc (Lmem ofs pt bf) ty1) (Eval (v2,vt2) ty2) ty =>
+            exists v2' t w' res,
+            ty = ty1 /\ sem_cast v2 ty2 ty1 tt = Some v2' /\
+              deref_loc ge ty1 m ofs pt bf t res /\ possible_trace w t w' /\
+              forall v1 vts lts ps1,
+                res ps = (Success (v1, vts, lts), ps1) ->
+                forall pct'' vt' lts' ps2,
+                  ('(pct',vt2') <- AssignT lc pct (EffectiveT lc vts) vt2;;
+                   StoreT lc pct' pt vt2' lts) ps1 = (Success (pct'', vt', lts'), ps2) ->
+                  exists t' w'' res',
+                    assign_loc ge ce ty1 m ofs pt lts' bf (v2',vt') t' res' /\ possible_trace w' t' w''
+        | Eassign (Eloc (Ltmp b) ty1) (Eval (v2,vt2) ty2) ty =>
+            exists v1 v2' vt1,
+            ty = ty1 /\ te!b = Some (v1,vt1) /\ sem_cast v2 ty2 ty1 tt = Some v2'
+        | Eassign (Eloc (Lifun _ _) _) (Eval _ _) ty => False
+        | Eassign (Eloc (Lefun _ _ _ _ _) _) (Eval _ _) ty => False
+        | Ecomma (Eval v ty1) r2 ty =>
+            typeof r2 = ty
+        | Eparen (Eval (v1,vt1) ty1) tycast ty =>
+            exists v, sem_cast v1 ty1 tycast tt = Some v
+        | Ecall (Eval (Vfptr b,vft) tyf) rargs ty =>
+            exprlist_all_values rargs ->
+            exists tyargs tyres cconv fd res ps',
+              Genv.find_funct ge (Vfptr b) = Some fd /\
+                classify_fun tyf = fun_case_f tyargs tyres cconv /\
+                type_of_fundef fd = Tfunction tyargs tyres cconv /\
+                cast_arguments lc pct ps vft tt rargs tyargs ps' res /\
+                ((exists pct' vl, res = Success (pct', vl)) \/
+                   (exists failure, res = Fail failure))
+        | Ecall (Eval (Vefptr ef tyargs tyres cc,vft) tyf) rargs ty =>
+            exprlist_all_values rargs ->
+            exists res ps',
+              cast_arguments lc pct ps vft tt rargs tyargs ps' res /\
+                ((exists pct' vl, res = Success (pct', vl)) \/
+                   (exists failure, res = Fail failure))
+        | Ecall (Eval (_,_) _) rargs ty =>
+            ~ exprlist_all_values rargs
+        | _ => True
+        end.
+
+      Lemma lred_invert:
+        forall lc l pct te m l' te' m' ps ps',
+          lred ge ce e lc l pct te m l' te' m' ps ps' -> invert_expr_prop lc l ps pct te m.
+      Proof.
+        induction 1; red; auto.
+        - right; left; exists base, pt; auto.
+        - right; right; left; split; auto; exists base, bound, pt, gv; auto.
+        - right; right; right; left; split; auto; exists b, pt; auto.
+        - right; right; right; right; split; auto; exists ef, tyargs, tyres, cc, pt; auto.
+        - eauto.
+        - exists p. intuition. exists co, delta, bf. split;auto.
+        - exists p. intuition. exists co, delta, bf; auto.
+      Qed.
+
+      Lemma lfailred_invert:
+        forall lc l pct te m tr failure ps ps',
+          lfailred ce lc l pct tr failure ps ps' -> invert_expr_prop lc l ps pct te m.
+      Proof.
+        induction 1; red; auto.
+        - exists p. intuition. exists co, delta, bf; auto.
+        - exists p. intuition. exists co, delta, bf; auto.
+      Qed.
+
+      Ltac chomp :=
+        match goal with
+        | [H: possible_trace _ (?t1 ++ ?t2) _ |- _] =>
+            let w' := fresh "w" in
+            let H1 := fresh "H" in
+            let H2 := fresh "H" in
+            apply possible_trace_app_inv in H;
+            destruct H as [w' [H1 H2]]
+        | [H1: ?v1 = ?v2, H2: ?v1 = ?v3 |- _] =>
+            rewrite H1 in H2; clear H1
+        | [H1: ?rule = Success _, H2: ?rule = Success _ |- _] =>
+            rewrite H1 in H2; inv H2
+        | [H: (Success _, _) = (Success _, _) |- _] =>
+            inv H
+        | [H: (Success _, _) = (Fail _, _) |- _ ] =>
+            inv H
+        | [H: (Fail _, _) = (Success _, _) |- _ ] =>
+            inv H
+        | [H: Some _ = Some _ |- _ ] =>
+            inv H
+        | [H1: forall _ _, ?ty <> Tpointer _ _, H2: ?ty = Tpointer _ _ |- _] =>
+            congruence
+        | [H1: ?r ?ps = (_, _), H2: ?r ?ps = (_, _) |- _] =>
+            rewrite H1 in H2; inv H2
+        | [ H: sem_cast _ _ _ _ = Some (Vptr ?ofs) |-
+              exists v ofs, sem_cast _ _ _ _ = Some v /\ _ /\ _ -> _ ] =>
+            exists (Vptr ofs), ofs
+        | _ => idtac
+        end.
+
+      Lemma rred_invert:
+        forall lc w' pct r te m t pct' r' te' m' ps ps',
+          rred ge ce lc pct r te m t pct' r' te' m' ps ps' ->
+          possible_trace w t w' ->
+          invert_expr_prop lc r ps pct te m.
+      Proof.
+        induction 1; intros; red; repeat doinv; auto; repeat (repeat chomp; try contradiction; eexists; eauto; intros).
+        - destruct ty1; destruct ty; try congruence; repeat (eexists; eauto; try contradiction).  
+        - destruct ty1; destruct ty; try congruence; repeat (eexists; eauto; try contradiction).  
+        - destruct ty1; try congruence; repeat (eexists; eauto; try contradiction).  
+        - destruct ty; try congruence; repeat (eexists; eauto; try contradiction).  
+        - destruct ty1; destruct ty; try congruence; repeat (eexists; eauto; try contradiction).  
+      Qed.
+    
+      Lemma rfailred_invert:
+        forall lc w' ps pct r te m tr failure ps',
+          rfailred ge ce lc pct r te m tr failure ps ps' ->
+          possible_trace w tr w' -> invert_expr_prop lc r ps pct te m.
+      Proof.
+        induction 1; intros; red; repeat doinv; auto;
+          repeat (repeat chomp; try contradiction; eexists; intuition eauto).
+        - destruct ty1; destruct ty; try congruence; repeat (eexists; eauto; try contradiction).
+        - destruct ty1; destruct ty; try congruence; repeat (eexists; eauto; try contradiction).
+        - destruct ty; try congruence; repeat (eexists; eauto; try contradiction).
+        - destruct ty1; destruct ty; try congruence; repeat (eexists; eauto; try contradiction).
+        - destruct ty1; try congruence; repeat (eexists; eauto; try contradiction).
+      Qed.
+    
+      Lemma callred_invert:
+        forall lc ps pct pct' fpt r fd args ty te m ps',
+          callred ge lc pct r m fd fpt args ty pct' ps ps' ->
+          invert_expr_prop lc r ps pct te m.
+      Proof.
+        intros. inv H; simpl.
+        - unfold find_funct in H0. inv H0. intros.
+          exists tyargs, tyres, cconv, fd, (Success (pct', args)), ps'. intuition.
+          left. exists pct', args; intuition congruence.
+        - intros. exists (Success (pct', args)), ps'. intuition. left. exists pct', args.
+          intuition congruence.
+      Qed.
+
+      Scheme context_ind2 := Minimality for context Sort Prop
+          with contextlist_ind2 := Minimality for contextlist Sort Prop.
+      Combined Scheme context_contextlist_ind from context_ind2, contextlist_ind2. 
+
+      Lemma invert_expr_context:
+        (forall from to C, context from to C ->
+                           forall lc a ps pct te m,
+                             invert_expr_prop lc a ps pct te m ->
+                             invert_expr_prop lc (C a) ps pct te m)
+        /\(forall from C, contextlist from C ->
+                          forall lc a ps pct te m,
+                            invert_expr_prop lc a ps pct te m ->
+                            ~exprlist_all_values (C a)).
+      Proof.
+        apply context_contextlist_ind; intros; try (exploit H0; [eauto|intros]); simpl; auto;
+          try (destruct (C a); unfold invert_expr_prop in *; auto; contradiction).
+        - destruct e1; auto; destruct (C a); destruct v; auto. destruct v0; auto; contradiction.
+        - destruct e1; auto.
+          destruct l; auto; destruct (C a); auto; destruct v; auto; inv H2.
+        - destruct e1; auto; destruct (C a); auto; destruct l; auto; contradiction.
+        - destruct e1; auto. repeat dodestr; auto; try eapply H0; eauto.
+          + intros. elim (H0 lc a ps pct te m); auto. 
+          + intros. elim (H0 lc a ps pct te m); auto.
+        - destruct e1; auto. eapply H0. eauto.
+      Qed.
+      
+      Lemma imm_safe_t_inv:
+        forall lc k a ps pct te m,
+          imm_safe_t ge ce e w k lc a ps pct te m ->
+          match a with
+          | Eloc _ _ => True
+          | Eval _ _ => True
+          | _ => invert_expr_prop lc a ps pct te m
+          end.
+      Proof.
+        destruct invert_expr_context as [A B].
+        intros. inv H; auto.
+        - assert (invert_expr_prop lc (C l) ps pct te m).
+          { eapply A; eauto. eapply lred_invert; eauto. }
+          red in H. destruct (C l); auto; contradiction.
+        - assert (invert_expr_prop lc (C l) ps pct te m).
+          { eapply A; eauto. eapply lfailred_invert; eauto. }
+          red in H. destruct (C l); auto; contradiction.
+        - assert (invert_expr_prop lc (C r) ps pct te m).
+          { eapply A; eauto. eapply rred_invert; eauto. }
+          red in H. destruct (C r); auto; contradiction.
+        - assert (invert_expr_prop lc (C r) ps pct te m).
+          { eapply A; eauto. eapply rfailred_invert; eauto. }
+          red in H. destruct (C r); auto; contradiction.
+        - assert (invert_expr_prop lc (C r) ps pct te m).
+          { eapply A; eauto. eapply callred_invert; eauto. }
+          red in H. destruct (C r); auto; contradiction.
+      Qed.
+      
+      (** Soundness: if [step_expr] returns [Some ll], then every element
+          of [ll] is a reduct. *)
+
+      Lemma context_compose:
+        forall k2 k3 C2, context k2 k3 C2 ->
+                         forall k1 C1, context k1 k2 C1 ->
+                                       context k1 k3 (fun x => C2(C1 x))
+      with contextlist_compose:
+        forall k2 C2, contextlist k2 C2 ->
+                      forall k1 C1, context k1 k2 C1 ->
+                                    contextlist k1 (fun x => C2(C1 x)).
+      Proof.
+        - induction 1; intros; try (constructor; eauto).
+          replace (fun x => C1 x) with C1. auto. apply extensionality; auto.
+        - induction 1; intros; constructor; eauto.
+      Qed.
+      
+      Local Hint Constructors context contextlist : core.
+      Local Hint Resolve context_compose contextlist_compose : core.
+      
+      Opaque do_deref_loc.
+      Opaque do_assign_loc.
+
+      Section REDUCTION_OK.
+
+        Definition reduction_ok (k: kind) (lc:Cabs.loc) (ps: pstate) (pct: control_tag)
+                   (a: expr) (te: tenv) (m: mem) (rd: reduction) : Prop :=
+          match k, rd with
+          | LV, Lred _ l' te' m' ps' => lred ge ce e lc a pct te m l' te' m' ps ps'
+          | RV, Rred _ pct' r' te' m' t ps' =>
+              rred ge ce lc pct a te m t pct' r' te' m' ps ps' /\ exists w', possible_trace w t w'
+          | RV, Callred _ fd fpt args tyres te' m' pct' ps' =>
+              callred ge lc pct a m fd fpt args tyres pct' ps ps' /\ te' = te /\ m' = m
+          | LV, Stuckred => ~imm_safe_t ge ce e w k lc a ps pct te m
+          | RV, Stuckred => ~imm_safe_t ge ce e w k lc a ps pct te m
+          | LV, Failstopred _ failure tr ps' => lfailred ce lc a pct tr failure ps ps'
+          | RV, Failstopred _ failure tr ps' => rfailred ge ce lc pct a te m tr failure ps ps' /\ exists w', possible_trace w tr w'
+          | _, _ => False
+          end.
+
+        Definition reducts_ok (k: kind) (lc:Cabs.loc) (ps: pstate) (pct: control_tag)
+                   (a: expr) (te: tenv) (m: mem) (ll: reducts expr) : Prop :=
+          (forall C rd,
+              In (C, rd) ll ->
+              exists a', exists k', context k' k C /\ a = C a' /\ reduction_ok k' lc ps pct a' te m rd)
+          /\ (ll = nil ->
+              match k with
+              | LV => is_loc a <> None
+              | RV => is_val a <> None
+              end).
+
+        Definition list_reducts_ok (lc:Cabs.loc) (ps: pstate) (pct: control_tag)
+                   (al: exprlist) (te: tenv) (m: mem) (ll: reducts exprlist) : Prop :=
+          (forall C rd,
+              In (C, rd) ll ->
+              exists a', exists k', contextlist k' C /\ al = C a' /\ reduction_ok k' lc ps pct a' te m rd)
+          /\ (ll = nil -> is_val_list al <> None).
+        
+      Lemma topred_ok:
+        forall k lc ps pct a m te rd,
+          reduction_ok k lc ps pct a te m rd ->
+          reducts_ok k lc ps pct a te m (topred rd).
+      Proof.
+        intros. unfold topred; split; simpl; intros.
+        destruct H0; try contradiction. inv H0. exists a; exists k; auto.
+        congruence.
+      Qed.
+
+      Lemma stuck_ok:
+        forall lc k a ps pct te m,
+          ~imm_safe_t ge ce e w k lc a ps pct te m ->
+          reducts_ok k lc ps pct a te m stuck.
+      Proof.
+        intros. unfold stuck; split; simpl; intros.
+        destruct H0; try contradiction. inv H0. exists a; exists k; intuition. red. destruct k; auto.
+        inv H0.
+      Qed.
+
+      Lemma wrong_kind_ok:
+        forall lc k ps pct a te m,
+          k <> expr_kind a ->
+          reducts_ok k lc ps pct  a te m stuck.
+      Proof.
+        intros. apply stuck_ok. red; intros. exploit imm_safe_kind; eauto.
+        eapply imm_safe_t_imm_safe; eauto.
+      Qed.
+
+      Lemma not_invert_ok:
+        forall lc k ps pct a te m,
+          match a with
+          | Eloc _ _ => False
+          | Eval _ _ => False
+          | _ => invert_expr_prop lc a ps pct te m -> False
+          end ->
+          reducts_ok k lc ps pct a te m stuck.
+      Proof.
+        intros. apply stuck_ok. red; intros.
+        exploit imm_safe_t_inv; eauto. destruct a; auto.
+      Qed.
+
+      Lemma incontext_ok:
+        forall lc k ps pct a te m C res k' a',
+          reducts_ok k' lc ps pct a' te m res ->
+          a = C a' ->
+          context k' k C ->
+          match k' with LV => is_loc a' = None | RV => is_val a' = None end ->
+          reducts_ok k lc ps pct a te m (incontext C res).
+      Proof.
+        unfold reducts_ok, incontext; intros. destruct H. split; intros.
+        exploit list_in_map_inv; eauto. intros [[C1 rd1] [P Q]]. inv P.
+        exploit H; eauto. intros [a'' [k'' [U [V W]]]].
+        exists a''; exists k''. split. eapply context_compose; eauto. rewrite V; auto.
+        destruct res; simpl in H4; try congruence. destruct k'; intuition congruence.
+      Qed.
+
+      Lemma incontext2_ok:
+        forall k lc ps pct a te m k1 a1 res1 k2 a2 res2 C1 C2,
+          reducts_ok k1 lc ps pct a1 te m res1 ->
+          reducts_ok k2 lc ps pct a2 te m res2 ->
+          a = C1 a1 -> a = C2 a2 ->
+          context k1 k C1 -> context k2 k C2 ->
+          match k1 with LV => is_loc a1 = None | RV => is_val a1 = None end
+          \/ match k2 with LV => is_loc a2 = None | RV => is_val a2 = None end ->
+          reducts_ok k lc ps pct a te m (incontext2 C1 res1 C2 res2).
+      Proof.
+        unfold reducts_ok, incontext2, incontext; intros. destruct H; destruct H0; split; intros.
+        destruct (in_app_or _ _ _ H8).
+        - exploit list_in_map_inv; eauto. intros [[C' rd'] [P Q]]. inv P.
+          exploit H; eauto. intros [a'' [k'' [U [V W]]]].
+          exists a''; exists k''. split. eapply context_compose; eauto. rewrite V; auto.
+        - exploit list_in_map_inv; eauto. intros [[C' rd'] [P Q]]. inv P.
+          exploit H0; eauto. intros [a'' [k'' [U [V W]]]].
+          exists a''; exists k''. split. eapply context_compose; eauto. rewrite H2; rewrite V; auto.
+        - destruct res1; simpl in H8; try congruence. destruct res2; simpl in H8; try congruence.
+          destruct H5. destruct k1; intuition congruence. destruct k2; intuition congruence.
+      Qed.
+
+      Lemma incontext2_list_ok:
+        forall lc ps pct a1 a2 ty te m res1 res2,
+          reducts_ok RV lc ps pct a1 te m res1 ->
+          list_reducts_ok lc ps pct a2 te m res2 ->
+          is_val a1 = None \/ is_val_list a2 = None ->
+          reducts_ok RV lc ps pct (Ecall a1 a2 ty) te m
+                     (incontext2 (fun x => Ecall x a2 ty) res1
+                                 (fun x => Ecall a1 x ty) res2).
+      Proof.
+        unfold reducts_ok, incontext2, incontext; intros. destruct H; destruct H0; split; intros.
+        destruct (in_app_or _ _ _ H4).
+        exploit list_in_map_inv; eauto. intros [[C' rd'] [P Q]]. inv P.
+        exploit H; eauto. intros [a'' [k'' [U [V W]]]].
+        exists a''; exists k''. split. eauto. rewrite V; auto.
+        exploit list_in_map_inv; eauto. intros [[C' rd'] [P Q]]. inv P.
+        exploit H0; eauto. intros [a'' [k'' [U [V W]]]].
+        exists a''; exists k''. split. eauto. rewrite V; auto.
+        destruct res1; simpl in H4; try congruence. destruct res2; simpl in H4; try congruence.
+        tauto.
+      Qed.
+
+      Lemma incontext2_list_ok':
+        forall lc ps pct a1 a2 te m res1 res2,
+          reducts_ok RV lc ps pct a1 te m res1 ->
+          list_reducts_ok lc ps pct a2 te m res2 ->
+          list_reducts_ok lc ps pct (Econs a1 a2) te m
+                          (incontext2 (fun x => Econs x a2) res1
+                                      (fun x => Econs a1 x) res2).
+      Proof.
+        unfold reducts_ok, list_reducts_ok, incontext2, incontext; intros.
+        destruct H; destruct H0. split; intros.
+        destruct (in_app_or _ _ _ H3).
+        exploit list_in_map_inv; eauto. intros [[C' rd'] [P Q]]. inv P.
+        exploit H; eauto. intros [a'' [k'' [U [V W]]]].
+        exists a''; exists k''. split. eauto. rewrite V; auto.
+        exploit list_in_map_inv; eauto. intros [[C' rd'] [P Q]]. inv P.
+        exploit H0; eauto. intros [a'' [k'' [U [V W]]]].
+        exists a''; exists k''. split. eauto. rewrite V; auto.
+        destruct res1; simpl in H3; try congruence. destruct res2; simpl in H3; try congruence.
+        simpl. destruct (is_val a1). destruct (is_val_list a2). congruence. intuition congruence. intuition congruence.
+      Qed.
+
+      Lemma is_val_list_all_values:
+        forall al vtl, is_val_list al = Some vtl -> exprlist_all_values al.
+      Proof.
+        induction al; simpl; intros; auto.
+        destruct (is_val r1) as [[[v vt] ty]|] eqn:?; try discriminate.
+        destruct (is_val_list al) as [vtl'|] eqn:?; try discriminate.
+        rewrite (is_val_inv _ _ _ Heqo). eauto.
+      Qed.
+
+      Definition is_pointer (ty : type) : option (type * attr) :=
+        match ty with
+        | Tpointer ty' attr => Some (ty', attr)
+        | _ => None
+        end.
+
+      Lemma is_pointer_inv :
+        forall ty ty' attr,
+          is_pointer ty = Some (ty', attr) ->
+          ty = Tpointer ty' attr.
+      Proof.
+        destruct ty; simpl; congruence.
+      Qed.
+
+      Ltac solve_trace :=
+        match goal with
+        | [ |- exists w', possible_trace ?w E0 w' ] => exists w; constructor
+        | [ H: possible_trace ?w1 ?tr ?w2 |- exists w3, possible_trace ?w1 ?tr w3 ] =>
+            exists w2; auto
+        | [ H1: possible_trace ?w1 ?tr1 ?w2, H2: possible_trace ?w2 ?tr2 ?w3
+            |- exists w', possible_trace ?w1 (?tr1 ++ ?tr2) w' ] =>
+            exists w3; eapply possible_trace_app; eauto
+        end.
+
+      Ltac inv_deref_assign :=
+        match goal with
+        | [ H: do_deref_loc _ _ _ _ _ _ _ = Some _ |- _ ] =>
+            eapply do_deref_loc_sound in H; intuition
+        | [ H: do_assign_loc _ _ _ _ _ _ _ _ _ _ = Some _ |- _ ] =>
+            eapply do_assign_loc_sound in H; intuition
+        end.
+
+      Ltac do_complete :=
+        match goal with
+        | [H: deref_loc _ _ _ _ _ _ _ _ |- _ ] =>
+            eapply do_deref_loc_complete in H; [|eauto]
+        | [H: assign_loc _ _ _ _ _ _ _ _ _ _ _ |- _ ] =>
+            eapply do_assign_loc_complete in H; [|eauto]
+        end.
+
+      Notation "'try' X , PS <- A ; 'catch' R , T ; B" :=
+        (tryred A (fun X PS => B) R T)
+          (at level 200, X pattern, PS name, A at level 100, B at level 200)
+          : reducts_monad_scope.
+
+      Open Scope reducts_monad_scope.
+
+      Ltac tag_destr :=
+        match goal with
+        | [ |- context [try _, _ <- ?e; catch _,_; _] ] =>
+            let r := fresh "r" in
+            let ps := fresh "ps" in
+            destruct e as [r ps] eqn:?;
+                                 destruct r; simpl
+        | [ |- context [try (_, _) , _ <- ?e; catch _,_; _] ] =>
+            let r := fresh "r" in
+            let ps := fresh "ps" in
+            destruct e as [r ps] eqn:?;
+                                 destruct r; simpl
+        end.
+
+      Ltac solve_rred red := eapply topred_ok; auto; split; [eapply red|solve_trace]; eauto.
+
+      Ltac solve_red :=
+        match goal with
+
+        (* Lred *)
+          
+        | [ |- reducts_ok _ _ _ _ _ _ _ (topred (Lred "red_var_tmp" _ _ _ _)) ] => 
+            eapply topred_ok; auto; eapply red_var_tmp; eauto
+        | [ |- reducts_ok _ _ _ _ _ _ _ (topred (Lred "red_var_local" _ _ _ _)) ] => 
+            eapply topred_ok; auto; eapply red_var_local; eauto
+        | [ |- reducts_ok _ _ _ _ _ _ _ (topred (Lred "red_func" _ _ _ _)) ] => 
+            eapply topred_ok; auto; eapply red_func; eauto
+        | [ |- reducts_ok _ _ _ _ _ _ _ (topred (Lred "red_ext_func" _ _ _ _)) ] => 
+            eapply topred_ok; auto; eapply red_ext_func; eauto
+        | [ |- reducts_ok _ _ _ _ _ _ _ (topred (Lred "red_builtin" _ _ _ _)) ] => 
+            eapply topred_ok; auto; eapply red_builtin; eauto
+        | [ |- reducts_ok _ _ _ _ _ _ _ (topred (Lred "red_var_global" _ _ _ _)) ] => 
+            eapply topred_ok; auto; eapply red_var_global; eauto
+        | [ |- reducts_ok _ _ _ _ _ _ _ (topred (Lred "red_field_struct" _ _ _ _)) ] => 
+            eapply topred_ok; auto; eapply red_field_struct; eauto
+        | [ |- reducts_ok _ _ _ _ _ _ _ (topred (Lred "red_field_union" _ _ _ _)) ] => 
+            eapply topred_ok; auto; eapply red_field_union; eauto
+        | [ |- reducts_ok _ _ _ _ _ _ _ (topred (Lred "red_deref" _ _ _ _)) ] => 
+            eapply topred_ok; auto; eapply red_deref; eauto
+
+        (* Lfailred *)
+                                                        
+        | [ |- reducts_ok _ _ _ _ _ _ _ (topred (Failstopred "failred_field_struct" _ _ _)) ] => 
+            eapply topred_ok; auto; eapply failred_field_struct; eauto
+        | [ |- reducts_ok _ _ _ _ _ _ _ (topred (Failstopred "failred_field_union" _ _ _)) ] => 
+            eapply topred_ok; auto; eapply failred_field_union; eauto
+
+        (* Rred *)
+                                                                  
+        | [ |- reducts_ok _ _ _ _ _ _ _ (topred (Rred "red_const"  _ _ _ _ _ _)) ] =>
+            solve_rred red_const
+        | [ |- reducts_ok _ _ _ _ _ _ _ (topred (Rred "red_rvalof_mem" _ _ _ _ _ _)) ] =>
+            repeat inv_deref_assign; solve_rred red_rvalof_mem
+        | [ |- reducts_ok _ _ _ _ _ _ _ (topred (Rred "red_rvalof_tmp" _ _ _ _ _ _)) ] =>
+            solve_rred red_rvalof_tmp
+        | [ |- reducts_ok _ _ _ _ _ _ _ (topred (Rred "red_rvalof_ifun" _ _ _ _ _ _)) ] =>
+            solve_rred red_rvalof_ifun
+        | [ |- reducts_ok _ _ _ _ _ _ _ (topred (Rred "red_rvalof_efun" _ _ _ _ _ _)) ] =>
+            solve_rred red_rvalof_efun
+        | [ |- reducts_ok _ _ _ _ _ _ _ (topred (Rred "red_addrof_loc" _ _ _ _ _ _)) ] =>
+            solve_rred red_addrof_loc
+        | [ |- reducts_ok _ _ _ _ _ _ _ (topred (Rred "red_addrof_fptr" _ _ _ _ _ _)) ] =>
+            solve_rred red_addrof_fptr
+        | [ |- reducts_ok _ _ _ _ _ _ _ (topred (Rred "red_addrof_efptr" _ _ _ _ _ _)) ] =>
+            solve_rred red_addrof_efptr
+        | [ |- reducts_ok _ _ _ _ _ _ _ (topred (Rred "red_unop" _ _ _ _ _ _)) ] =>
+            solve_rred red_unop
+        | [ |- reducts_ok _ _ _ _ _ _ _ (topred (Rred "red_binop" _ _ _ _ _ _)) ] =>
+            solve_rred red_binop
+        | [ |- reducts_ok _ _ _ _ _ _ _ (topred (Rred "red_seqand_true" _ _ _ _ _ _)) ] =>
+            solve_rred red_seqand_true
+        | [ |- reducts_ok _ _ _ _ _ _ _ (topred (Rred "red_seqand_false" _ _ _ _ _ _)) ] =>
+            solve_rred red_seqand_false
+        | [ |- reducts_ok _ _ _ _ _ _ _ (topred (Rred "red_seqor_true" _ _ _ _ _ _)) ] =>
+            solve_rred red_seqor_true
+        | [ |- reducts_ok _ _ _ _ _ _ _ (topred (Rred "red_seqor_false" _ _ _ _ _ _)) ] =>
+            solve_rred red_seqor_false
+        | [ |- reducts_ok _ _ _ _ _ _ _ (topred (Rred "red_condition" _ _ _ _ _ _)) ] =>
+            solve_rred red_condition
+        | [ |- reducts_ok _ _ _ _ _ _ _ (topred (Rred "red_sizeof" _ _ _ _ _ _)) ] =>
+            solve_rred red_sizeof
+        | [ |- reducts_ok _ _ _ _ _ _ _ (topred (Rred "red_assign_mem" _ _ _ _ _ _)) ] =>
+            repeat inv_deref_assign; solve_rred red_assign_mem
+        | [ |- reducts_ok _ _ _ _ _ _ _ (topred (Rred "red_assign_tmp" _ _ _ _ _ _)) ] =>
+            solve_rred red_assign_tmp
+        | [ |- reducts_ok _ _ _ _ _ _ _ (topred (Rred "red_assignop_mem" _ _ _ _ _ _)) ] =>
+            repeat inv_deref_assign; solve_rred red_assignop_mem
+        | [ |- reducts_ok _ _ _ _ _ _ _ (topred (Rred "red_assignop_tmp" _ _ _ _ _ _)) ] =>
+            solve_rred red_assignop_tmp
+        | [ |- reducts_ok _ _ _ _ _ _ _ (topred (Rred "red_assignop_ifun" _ _ _ _ _ _)) ] =>
+            solve_rred red_assignop_ifun
+        | [ |- reducts_ok _ _ _ _ _ _ _ (topred (Rred "red_assignop_efun" _ _ _ _ _ _)) ] =>
+            solve_rred red_assignop_efun
+        | [ |- reducts_ok _ _ _ _ _ _ _ (topred (Rred "red_postincr_mem" _ _ _ _ _ _)) ] =>
+            repeat inv_deref_assign; solve_rred red_postincr_mem
+        | [ |- reducts_ok _ _ _ _ _ _ _ (topred (Rred "red_postincr_tmp" _ _ _ _ _ _)) ] =>
+            solve_rred red_postincr_tmp
+        | [ |- reducts_ok _ _ _ _ _ _ _ (topred (Rred "red_postincr_ifun" _ _ _ _ _ _)) ] =>
+            solve_rred red_postincr_ifun
+        | [ |- reducts_ok _ _ _ _ _ _ _ (topred (Rred "red_postincr_efun" _ _ _ _ _ _)) ] =>
+            solve_rred red_postincr_efun
+        | [ |- reducts_ok _ _ _ _ _ _ _ (topred (Rred "red_alignof" _ _ _ _ _ _)) ] =>
+            solve_rred red_alignof
+        | [ |- reducts_ok _ _ _ _ _ _ _ (topred (Rred "red_comma" _ _ _ _ _ _)) ] =>
+            solve_rred red_comma
+        | [ |- reducts_ok _ _ _ _ _ _ _ (topred (Rred "red_paren" _ _ _ _ _ _)) ] =>
+            solve_rred red_paren
+        | [ |- reducts_ok _ _ _ _ _ _ _ (topred (Rred "red_cast_int_int" _ _ _ _ _ _)) ] =>
+            solve_rred red_cast_int_int
+        | [ |- reducts_ok _ _ _ _ _ _ _ (topred (Rred "red_cast_ptr_int" _ _ _ _ _ _)) ] =>
+            repeat inv_deref_assign; solve_rred red_cast_ptr_int
+        | [ |- reducts_ok _ _ _ _ _ _ _ (topred (Rred "red_cast_int_ptr" _ _ _ _ _ _)) ] =>
+            repeat inv_deref_assign; solve_rred red_cast_int_ptr
+        | [ |- reducts_ok _ _ _ _ _ _ _ (topred (Rred "red_cast_int_nullptr" _ _ _ _ _ _)) ] =>
+            solve_rred red_cast_int_nullptr
+        | [ |- reducts_ok _ _ _ _ _ _ _ (topred (Rred "red_cast_ptr_ptr" _ _ _ _ _ _)) ] =>
+            repeat inv_deref_assign; solve_rred red_cast_ptr_ptr
+        | [ |- reducts_ok _ _ _ _ _ _ _ (topred (Rred "red_cast_ptr_nullptr" _ _ _ _ _ _)) ] =>
+            solve_rred red_cast_ptr_nullptr
+                                                                   
+        (* Rfailred *)
+
+        | [ |- reducts_ok _ _ _ _ _ _ _ (topred (Failstopred "failred_const" _ _ _)) ] =>
+            solve_rred failred_const
+        | [ |- reducts_ok _ _ _ _ _ _ _ (topred (Failstopred "failred_rvalof_mem0" _ _ _)) ] =>
+            repeat inv_deref_assign; solve_rred failred_rvalof_mem0
+        | [ |- reducts_ok _ _ _ _ _ _ _ (topred (Failstopred "failred_rvalof_mem1" _ _ _)) ] =>
+            repeat inv_deref_assign; solve_rred failred_rvalof_mem1
+        | [ |- reducts_ok _ _ _ _ _ _ _ (topred (Failstopred "failred_rvalof_tmp" _ _ _)) ] =>
+            solve_rred failred_rvalof_tmp
+        | [ |- reducts_ok _ _ _ _ _ _ _ (topred (Failstopred "failred_unop" _ _ _)) ] =>
+            solve_rred failred_unop
+        | [ |- reducts_ok _ _ _ _ _ _ _ (topred (Failstopred "failred_binop" _ _ _)) ] =>
+            solve_rred failred_binop
+        | [ |- reducts_ok _ _ _ _ _ _ _ (topred (Failstopred "failred_seqand" _ _ _)) ] =>
+            solve_rred failred_seqand
+        | [ |- reducts_ok _ _ _ _ _ _ _ (topred (Failstopred "failred_seqor" _ _ _)) ] =>
+            solve_rred failred_seqor
+        | [ |- reducts_ok _ _ _ _ _ _ _ (topred (Failstopred "failred_condition" _ _ _)) ] =>
+            solve_rred failred_condition
+        | [ |- reducts_ok _ _ _ _ _ _ _ (topred (Failstopred "failred_sizeof" _ _ _)) ] =>
+            solve_rred failred_sizeof
+        | [ |- reducts_ok _ _ _ _ _ _ _ (topred (Failstopred "failred_alignof" _ _ _)) ] =>
+            solve_rred failred_alignof
+        | [ |- reducts_ok _ _ _ _ _ _ _ (topred (Failstopred "failred_assign_mem0" _ _ _)) ] =>
+            repeat inv_deref_assign; solve_rred failred_assign_mem0
+        | [ |- reducts_ok _ _ _ _ _ _ _ (topred (Failstopred "failred_assign_mem1" _ _ _)) ] =>
+            repeat inv_deref_assign; solve_rred failred_assign_mem1
+        | [ |- reducts_ok _ _ _ _ _ _ _ (topred (Failstopred "failred_assign_mem2" _ _ _)) ] =>
+            repeat inv_deref_assign; solve_rred failred_assign_mem2
+        | [ |- reducts_ok _ _ _ _ _ _ _ (topred (Failstopred "failred_assign_tmp" _ _ _)) ] =>
+            solve_rred failred_assign_tmp
+        | [ |- reducts_ok _ _ _ _ _ _ _ (topred (Failstopred "failred_assignop_mem0" _ _ _)) ] =>
+            repeat inv_deref_assign; solve_rred failred_assignop_mem0
+        | [ |- reducts_ok _ _ _ _ _ _ _ (topred (Failstopred "failred_assignop_mem1" _ _ _)) ] =>
+            repeat inv_deref_assign; solve_rred failred_assignop_mem1
+        | [ |- reducts_ok _ _ _ _ _ _ _ (topred (Failstopred "failred_assignop_tmp" _ _ _)) ] =>
+            solve_rred failred_assignop_tmp
+        | [ |- reducts_ok _ _ _ _ _ _ _ (topred (Failstopred "failred_postincr_mem0" _ _ _)) ] =>
+            repeat inv_deref_assign; solve_rred failred_postincr_mem0
+        | [ |- reducts_ok _ _ _ _ _ _ _ (topred (Failstopred "failred_postincr_mem1" _ _ _)) ] =>
+            repeat inv_deref_assign; solve_rred failred_postincr_mem1
+        | [ |- reducts_ok _ _ _ _ _ _ _ (topred (Failstopred "failred_postincr_tmp" _ _ _)) ] =>
+            solve_rred failred_postincr_tmp
+        | [ |- reducts_ok _ _ _ _ _ _ _ (topred (Failstopred "failred_paren" _ _ _)) ] =>
+            solve_rred failred_paren
+        | [ |- reducts_ok _ _ _ _ _ _ _ (topred (Failstopred "failred_cast_int_int" _ _ _)) ] =>
+            solve_rred failred_cast_int_int
+        | [ |- reducts_ok _ _ _ _ _ _ _ (topred (Failstopred "failred_cast_ptr_int" _ _ _)) ] =>
+            repeat inv_deref_assign; solve_rred failred_cast_ptr_int
+        | [ |- reducts_ok _ _ _ _ _ _ _ (topred (Failstopred "failred_cast_int_ptr" _ _ _)) ] =>
+            repeat inv_deref_assign; solve_rred failred_cast_int_ptr
+        | [ |- reducts_ok _ _ _ _ _ _ _ (topred (Failstopred "failred_cast_int_nullptr" _ _ _)) ] =>
+            solve_rred failred_cast_int_nullptr
+        | [ |- reducts_ok _ _ _ _ _ _ _ (topred (Failstopred "failred_cast_ptr_ptr" _ _ _)) ] =>
+            repeat inv_deref_assign; solve_rred failred_cast_ptr_ptr
+        | [ |- reducts_ok _ _ _ _ _ _ _ (topred (Failstopred "failred_cast_ptr_nullptr" _ _ _)) ] =>
+            solve_rred failred_cast_ptr_nullptr
+        | [ |- reducts_ok _ _ _ _ _ _ _ (topred (Failstopred "red_call_internal_fail" _ _ _)) ] =>
+            eapply topred_ok; split; [eapply red_call_internal_fail; eauto | solve_trace]
+        | [ |- reducts_ok _ _ _ _ _ _ _ (topred (Failstopred "red_call_external_fail" _ _ _)) ] =>
+            eapply topred_ok; split; [eapply red_call_external_fail; eauto | solve_trace]
+
+        (* Callred *)
+        | [ |- reducts_ok _ _ _ _ _ _ _ (topred (Callred "red_call_internal" _ _ _ _ _ _ _ _)) ] =>
+            eapply topred_ok; auto; split; eauto; eapply red_call_internal; eauto
+        | [ |- reducts_ok _ _ _ _ _ _ _ (topred (Callred "red_call_external" _ _ _ _ _ _ _ _)) ] =>
+            eapply topred_ok; auto; split; [eapply red_call_external|auto]
+                                             
+        | [ |- reducts_ok _ _ _ _ _ _ _ (incontext _ _) ] =>
+            eapply incontext_ok; eauto
+        | [ |- reducts_ok _ _ _ _ _ _ _ (incontext2 _ _ _ (step_expr _ _ _ _ _ _ _ _ _ _ _)) ] =>
+            eapply incontext2_ok; eauto
+        | [ |- reducts_ok _ _ _ _ _ _ _ (incontext2 _ _ _ _) ] =>
+            eapply incontext2_list_ok; eauto
+        end.
+
+      Ltac solve_nullptr :=
+        match goal with
+        | [ |- Vnullptr (Vptr _)] =>
+            constructor; unfold concretize; lia
+        | [ |- ~ Vnullptr (Vptr _)] =>
+            let H := fresh "H" in
+            intro H; inv H; unfold concretize in *; lia
+        end.
+
+      
+      Lemma step_cast_sound_ptr_ptr:
+        forall lc ps pct v vt ty ty1 attr attr1 te m,
+          reducts_ok RV lc ps pct (Ecast (Eval (v,vt) (Tpointer ty attr)) (Tpointer ty1 attr1)) te m
+                     (step_expr ge ce e w RV lc ps pct (Ecast (Eval (v,vt) (Tpointer ty attr)) (Tpointer ty1 attr1)) te m).
+      Admitted.
+(*      Proof.
+        intros. unfold step_expr; simpl.
+        repeat dodestr; repeat doinv; repeat chomp; repeat tag_destr; subst; try solve_red;
+          try solve_nullptr.
+        - exists p1. intuition eauto.  
+        - exists p1. intuition eauto.  
+        - apply not_invert_ok; simpl; intros; repeat doinv.
+          inv H. inv Heqo. repeat chomp.
+          destruct H0. 
+          { intro. inv H. unfold concretize in H1. rewrite H1 in Heqb.
+            simpl in Heqb. discriminate. }
+          repeat doinv.
+          do_complete.
+          repeat chomp.
+        - apply not_invert_ok; simpl; intros; repeat doinv.    
+          inv H. inv Heqo. repeat chomp.
+          destruct H0.
+          { intro. inv H. unfold concretize in H1. rewrite H1 in Heqb. simpl in Heqb. discriminate. }
+          repeat doinv.
+          do_complete.
+          repeat chomp. discriminate.
+        - apply not_invert_ok; simpl; intros; repeat doinv.    
+          inv H. inv Heqo. inv Heqo0. repeat chomp.
+          unfold is_ptr in H3. discriminate.
+        - apply not_invert_ok; simpl; intros; repeat doinv.    
+          inv H. inv Heqo. repeat chomp. discriminate.
+      Qed. *)
+
+      Lemma step_cast_sound_ptr_to:
+        forall lc ps pct v vt ty ty1 attr te m,
+          reducts_ok RV lc ps pct (Ecast (Eval (v,vt) (Tpointer ty attr)) ty1) te m
+                     (step_expr ge ce e w RV lc ps pct (Ecast (Eval (v,vt) (Tpointer ty attr)) ty1) te m).
+      Proof with apply not_invert_ok; simpl; intros; repeat doinv; repeat chomp; discriminate.
+        intros. destruct ty1.
+        5: apply step_cast_sound_ptr_ptr.
+        all: unfold step_expr; simpl;
+          repeat dodestr; repeat tag_destr; repeat doinv; try solve_red; try congruence;
+          try reflexivity...
+      Qed.
+        
+        Lemma step_cast_sound_to_ptr:
+          forall lc ps pct v vt ty ty1 attr te m,
+            reducts_ok RV lc ps pct (Ecast (Eval (v,vt) ty) (Tpointer ty1 attr)) te m
+                       (step_expr ge ce e w RV lc ps pct (Ecast (Eval (v,vt) ty) (Tpointer ty1 attr)) te m).
+        Admitted.
+        (*Proof with try (apply not_invert_ok; simpl; intros; repeat doinv; repeat chomp; discriminate).
+          intros. destruct ty...
+          3: apply step_cast_sound_ptr_ptr.
+          - unfold step_expr; simpl;
+              repeat dodestr; repeat tag_destr; repeat doinv; repeat chomp; try solve_red;
+              try congruence; try solve_nullptr...
+            + exists p1; intuition eauto.
+            + exists p1; intuition eauto.
+            + apply not_invert_ok; simpl; intros; repeat doinv; repeat chomp.
+              destruct H0; try solve_nullptr; repeat doinv.
+              do_complete. repeat chomp.
+            + apply not_invert_ok; simpl; intros; repeat doinv; repeat chomp.
+              destruct H0; try solve_nullptr; repeat doinv.
+              do_complete. repeat chomp. discriminate.
+          - unfold step_expr; simpl;
+              repeat dodestr; repeat tag_destr; repeat doinv; repeat chomp; try solve_red;
+              try congruence; try solve_nullptr...
+            + exists p1; intuition eauto.
+            + exists p1; intuition eauto.
+            + apply not_invert_ok; simpl; intros; repeat doinv; repeat chomp.
+              destruct H0; try solve_nullptr; repeat doinv.
+              do_complete. repeat chomp.
+            + apply not_invert_ok; simpl; intros; repeat doinv; repeat chomp.
+              destruct H0; try solve_nullptr; repeat doinv.
+              do_complete. repeat chomp. discriminate.
+          - unfold step_expr; simpl;
+              repeat dodestr; repeat tag_destr; repeat doinv; repeat chomp; try solve_red;
+              try congruence; try solve_nullptr...
+            + exists p1; intuition eauto.
+            + exists p1; intuition eauto.
+            + apply not_invert_ok; simpl; intros; repeat doinv; repeat chomp.
+              destruct H0; try solve_nullptr; repeat doinv.
+              do_complete. repeat chomp.
+            + apply not_invert_ok; simpl; intros; repeat doinv; repeat chomp.
+              destruct H0; try solve_nullptr; repeat doinv.
+              do_complete. repeat chomp. discriminate.
+          - unfold step_expr; simpl;
+              repeat dodestr; repeat tag_destr; repeat doinv; repeat chomp; try solve_red;
+              try congruence; try solve_nullptr...
+            + exists p1; intuition eauto.
+            + exists p1; intuition eauto.
+            + apply not_invert_ok; simpl; intros; repeat doinv; repeat chomp.
+              destruct H0; try solve_nullptr; repeat doinv.
+              do_complete. repeat chomp.
+            + apply not_invert_ok; simpl; intros; repeat doinv; repeat chomp.
+              destruct H0; try solve_nullptr; repeat doinv.
+              do_complete. repeat chomp. discriminate.
+        Qed. *)
+
+        Lemma step_cast_sound:
+          forall lc ps pct v vt ty ty1 te m,
+            reducts_ok RV lc ps pct (Ecast (Eval (v,vt) ty) ty1) te m
+                       (step_expr ge ce e w RV lc ps pct (Ecast (Eval (v,vt) ty) ty1) te m).
+        Proof.
+          intros. destruct ty.
+          5: apply step_cast_sound_ptr_to.
+          all: destruct ty1; try apply step_cast_sound_to_ptr.
+          all: unfold step_expr; simpl.
+          all: repeat dodestr; repeat tag_destr; repeat doinv.
+          all: try solve_red; try congruence; try reflexivity.
+          all: try apply not_invert_ok; simpl; intros; repeat doinv.
+          all: try congruence.
+          all: inv H.
+        Qed.
+
+        Theorem step_expr_sound:
+          forall lc ps pct a k te m,
+            reducts_ok k lc ps pct a te m (step_expr ge ce e w k lc ps pct a te m)
+            with step_exprlist_sound:
+              forall lc ps pct al te m,
+                list_reducts_ok lc ps pct al te m (step_exprlist ge ce e w lc ps pct al te m).
+        Proof with
+          (try (apply not_invert_ok; simpl; intros; repeat doinv;
+                try do_complete; intuition congruence; fail)).
+          Local Opaque incontext.
+          Local Opaque incontext2.
+          - clear step_expr_sound.
+            induction a; intros; cbn; simpl; destruct k;
+              try (apply wrong_kind_ok; simpl; congruence).
+            + (* Eval *)
+              split; intros. tauto. simpl; congruence.
+            + (* Evar *)
+              repeat dodestr; repeat doinv; subst; try solve_red...
+              destruct s; repeat dodestr; repeat doinv; subst; try solve_red...  
+            + (* Econst *)
+              repeat dodestr; repeat tag_destr; repeat doinv; subst; try solve_red...
+            + (* Efield *)
+              repeat dodestr; repeat tag_destr; repeat doinv; subst; try solve_red...
+            + (* Evalof *)
+              repeat dodestr; repeat tag_destr; repeat doinv; subst; try solve_red...
+              destruct (p3 ps) eqn:?; destruct r; simpl;
+                repeat dodestr; repeat tag_destr; repeat doinv; subst; try solve_red;
+                exists p3; intuition eauto. 
+            + (* Ederef *)
+              repeat dodestr; repeat tag_destr; repeat doinv; repeat chomp; subst; try solve_red...
+            + (* Eaddrof *)
+              repeat dodestr; repeat tag_destr; repeat doinv; subst; try solve_red...
+            + (* Eunop *)
+              repeat dodestr; repeat tag_destr; repeat doinv; subst; try solve_red...
+            + (* Ebinop *)
+              repeat dodestr; repeat tag_destr; repeat doinv; subst; try solve_red...
+            + (* Ecast *)
+              destruct a.
+              { destruct v as [v vt]. eapply step_cast_sound. }
+              all: simpl; solve_red; reflexivity.
+            + (* Eseqand *)
+              repeat dodestr; repeat tag_destr; repeat doinv; subst; try solve_red...
+            + (* Eseqor *)
+              repeat dodestr; repeat tag_destr; repeat doinv; subst; try solve_red...
+            + (* Econdition *)
+              repeat dodestr; repeat tag_destr; repeat doinv; subst; try solve_red...
+              * pose (b := true).
+                replace a2 with (if b then a2 else a3) at 2 by auto.
+                solve_red.
+              * pose (b := false).
+                replace a3 with (if b then a2 else a3) at 2 by auto.
+                solve_red.
+            + (* Esizeof *)
+              repeat dodestr; repeat tag_destr; repeat doinv; subst; try solve_red...
+            + (* Ealignof *)
+              repeat dodestr; repeat tag_destr; repeat doinv; subst; try solve_red...
+            + (* Eassign *)
+              repeat dodestr; repeat tag_destr; repeat doinv; subst; try solve_red...
+              destruct (p4 ps) eqn:?; destruct r; subst; simpl. 
+              unfold bind_res. repeat dodestr; repeat doinv; simpl.
+              * destruct (StoreT lc c pt v3 l (p2,l1)) eqn:?;
+                         destruct r; subst; simpl; repeat dodestr; repeat doinv; try solve_red;
+                  repeat cronch.
+                -- destruct (p7 (p0,l4)) eqn:?; destruct r; subst; simpl;
+                     repeat dodestr; repeat doinv; try solve_red; simpl; unfold bind_res;
+                     repeat (cronch; eauto).
+                -- apply not_invert_ok; simpl; intros; repeat doinv; repeat do_complete; repeat chomp.
+                   edestruct H3; eauto; repeat doinv; unfold bind_res; repeat (cronch; eauto).
+                   repeat do_complete; repeat chomp; discriminate.
+                -- simpl. unfold bind_res. repeat (cronch; eauto).
+              * solve_red; simpl; unfold bind_res; repeat cronch; auto.
+              * solve_red; simpl; unfold bind_res; repeat cronch; auto.
+            + (* Eassignop *)
+              repeat dodestr; repeat doinv; subst; try solve_red...
+              * destruct (p4 ps) eqn:?; destruct r; subst; simpl; unfold bind_res;
+                  repeat dodestr; repeat tag_destr; repeat doinv; try solve_red;
+                  simpl; unfold bind_res; repeat (cronch; eauto).
+              * tag_destr; solve_red.
+            + (* Epostincr *)
+              repeat dodestr; repeat doinv; subst; try solve_red...
+              * destruct (p3 ps) eqn:?; destruct r; subst; simpl; unfold bind_res;
+                  repeat dodestr; repeat tag_destr; repeat doinv; try solve_red;
+                  simpl; unfold bind_res; repeat (cronch; eauto).
+              * tag_destr; solve_red.
+              * destruct (p3 ps) eqn:?; destruct r; subst; simpl; unfold bind_res;
+                  repeat dodestr; repeat tag_destr; repeat doinv; try solve_red;
+                  simpl; unfold bind_res; repeat (cronch; eauto).
+              * tag_destr; solve_red.
+            + (* Ecomma *)
+              repeat dodestr; repeat tag_destr; repeat doinv; subst; try solve_red...
+            + (* Ecall *)
+              destruct (is_val a) as [[[vf fpt] fty]|] eqn:?; [destruct vf|];
+                (destruct (is_val_list rargs) as [vtl|] eqn:?;
+                                                        [exploit is_val_list_all_values;eauto;intros|]); try solve_red...
+              * repeat dodestr; repeat tag_destr; repeat doinv.
+                all: try (apply not_invert_ok; simpl; intros; repeat doinv;
+                          destruct H0; auto; repeat doinv; congruence).
+                -- solve_red. eapply sem_cast_arguments_sound; eauto.
+                -- solve_red. eapply sem_cast_arguments_sound; eauto.
+                -- eapply not_invert_ok; simpl; intros; repeat doinv.
+                   destruct H0; auto. repeat doinv.
+                   ++ eapply sem_cast_arguments_complete in H3. repeat doinv. congruence.
+                   ++ eapply sem_cast_arguments_complete in H3. repeat doinv. congruence.
+              * repeat dodestr; repeat tag_destr; repeat doinv.
+                -- solve_red. eapply sem_cast_arguments_sound; eauto.
+                -- solve_red. eapply sem_cast_arguments_sound; eauto.
+                -- apply not_invert_ok; simpl; intros; repeat doinv.
+                   destruct H0; auto.
+                   ++ repeat doinv; eapply sem_cast_arguments_complete in H0;
+                        repeat doinv; congruence.
+            + (* Ebuiltin *)
+              solve_red.
+            + (* loc *)
+              split; intros. tauto. simpl; congruence.
+            + (* paren *)
+              repeat dodestr; repeat tag_destr; repeat doinv; try solve_red...
+              
+          - clear step_exprlist_sound. induction al; simpl; intros.
+            + (* nil *)
+              split; intros. tauto. simpl; congruence.
+            + (* cons *)
+              eapply incontext2_list_ok'; eauto.
+        Qed.
+              
+      End REDUCTION_OK.
+
+      Ltac do_complete :=
+        match goal with
+        | [H: deref_loc _ _ _ _ _ _ _ _ |- _ ] =>
+            eapply do_deref_loc_complete in H; [|eauto]
+        | [H: assign_loc _ _ _ _ _ _ _ _ _ _ _ |- _ ] =>
+            eapply do_assign_loc_complete in H; [|eauto]
+        end.
+
+      Lemma step_exprlist_val_list:
+        forall lc te m ps pct al, is_val_list al <> None ->
+                                  step_exprlist ge ce e w lc ps pct al te m = nil.
+      Proof.
+        induction al; cbn; intros.
+        auto.
+        destruct (is_val r1) as [[v1 ty1]|] eqn:?; try congruence.
+        destruct (is_val_list al) eqn:?; try congruence.
+        rewrite (is_val_inv _ _ _ Heqo).
+        rewrite IHal. auto. congruence.
+      Qed.
+
+      (** Completeness part 1: [step_expr] contains all possible non-stuck reducts. *)
+      Lemma lred_topred:
+        forall lc ps pct l1 te m l2 te' m' ps',
+          lred ge ce e lc l1 pct te m l2 te' m' ps ps' ->
+          exists rule, step_expr ge ce e w LV lc ps pct l1 te m = topred (Lred rule l2 te' m' ps').
+      Proof.
+        induction 1; cbn.
+        (* var tmp *)
+        - rewrite H. rewrite dec_eq_true. econstructor; eauto.
+        (* var local *)
+        - rewrite H. rewrite dec_eq_true. econstructor; eauto.
+        (* var global *)
+        - rewrite H; rewrite H0. econstructor; eauto.
+        (* var ifun *)
+        - rewrite H; rewrite H0. econstructor; eauto.
+        (* var efun *)
+        - rewrite H; rewrite H0. econstructor; eauto.
+        (* builtin *)
+        - econstructor; eauto.
+        (* deref *)
+        - rewrite H. econstructor; eauto.
+        (* field struct *)
+        - rewrite H, H0, H1. simpl. eauto.
+        (* field union *)
+        - rewrite H, H0, H1. simpl. eauto.
+      Qed.
+
+      Lemma lfailred_topred:
+        forall lc ps pct l1 tr failure te m ps',
+          lfailred ce lc l1 pct tr failure ps ps' ->
+          exists rule, step_expr ge ce e w LV lc ps pct l1 te m = topred (Failstopred rule failure E0 ps').
+      Proof.
+        induction 1; cbn.
+        - rewrite H. rewrite H1. rewrite H0. eexists. constructor.
+        - rewrite H. rewrite H1. rewrite H0. eexists. constructor.
+      Qed.
+
+      Lemma rred_topred:
+        forall lc w' ps pct1 r1 te1 m1 t pct2 r2 te2 m2 ps',
+          rred ge ce lc pct1 r1 te1 m1 t pct2 r2 te2 m2 ps ps' -> possible_trace w t w' ->
+          exists rule, step_expr ge ce e w RV lc ps pct1 r1 te1 m1 = topred (Rred rule pct2 r2 te2 m2 t ps').
+      Proof.
+        induction 1; cbn; intros; eexists; unfold atom in *;
+          repeat doinv; repeat cronch; try constructor; auto.
+        - do_complete; eauto. rewrite H2.
+          rewrite RES. simpl. simpl in H0. rewrite H0.
+          reflexivity.
+        - destruct ty1; destruct ty; repeat cronch; eauto; congruence.
+        - subst. do_complete; eauto.
+          assert (Int64.unsigned p =? 0 = false)%Z.
+          { destruct (Int64.unsigned p) eqn:?; auto. exfalso. elim H2.
+            constructor. unfold concretize. auto. }
+          destruct ty1; repeat cronch; simpl; rewrite H0; repeat cronch; auto.
+          exfalso. eapply H. reflexivity.
+        - subst. inv H2. unfold concretize in H4. rewrite H4.      
+          destruct ty1; repeat cronch; simpl; auto.
+          exfalso. eapply H. reflexivity.
+        - subst. destruct ty; repeat cronch; simpl; auto.
+          exfalso. eapply H0. reflexivity.
+        - subst. eapply do_deref_loc_complete in H6; eauto.
+          assert (Int64.unsigned p =? 0 = false)%Z.
+          { destruct (Int64.unsigned p) eqn:?; auto. exfalso. elim H2.
+            constructor. unfold concretize. auto. }
+          simpl; repeat cronch; rewrite H; auto.
+        - subst. inv H2. unfold concretize in H0. rewrite H0. simpl; repeat cronch; simpl; eauto.
+        - eapply do_deref_loc_complete in H0; eauto.
+          eapply do_assign_loc_complete in H4; eauto.
+          repeat doinv; repeat cronch; eauto. simpl in H1. rewrite H1. simpl.
+          repeat cronch. eauto.
+        - eapply do_deref_loc_complete in H2; eauto.
+          repeat doinv; repeat cronch; eauto. simpl in H0. rewrite H0. simpl. eauto.
+        - eapply do_deref_loc_complete in H3; eauto.
+          repeat cronch.
+          simpl in H1. rewrite H1. simpl. rewrite H0. eauto.
+       Qed.
+      
+      Lemma rfailred_topred:
+        forall lc w' ps pct r1 tr failure te m ps',
+          rfailred ge ce lc pct r1 te m tr failure ps ps' -> possible_trace w tr w' ->
+          exists rule, step_expr ge ce e w RV lc ps pct r1 te m =
+                         topred (Failstopred rule failure tr ps').
+      Proof.
+        induction 1; cbn; intros; eexists; unfold atom in *;
+          repeat doinv; repeat cronch; try constructor; eauto.
+        - do_complete. repeat cronch. constructor.
+        - do_complete. inv H0. repeat cronch. constructor.
+        - do_complete. repeat cronch. constructor.
+        - do_complete. inv H1. repeat cronch. constructor.
+        - do_complete. inv H1. repeat cronch. do_complete. repeat cronch. constructor.
+        - do_complete. repeat cronch. constructor.
+        - do_complete. inv H0. repeat cronch. constructor.
+        - do_complete. repeat cronch. constructor.
+        - do_complete. inv H0. repeat cronch. constructor.
+        - destruct ty1; destruct ty; try congruence; repeat cronch; constructor.
+        - subst. do_complete.
+          assert (Int64.unsigned p =? 0 = false)%Z.
+          { destruct (Int64.unsigned p) eqn:?; auto.
+            elim H2. constructor. unfold concretize. auto. }
+          destruct ty1; repeat cronch; simpl; rewrite H0; repeat cronch; auto.
+          exfalso. eapply H. reflexivity.
+        - destruct ty; auto. eelim H0. reflexivity.
+        - subst. do_complete. simpl.
+          assert (Int64.unsigned p =? 0 = false)%Z.
+          { destruct (Int64.unsigned p) eqn:?; auto.
+            elim H2. constructor. unfold concretize. auto. }
+          rewrite H. repeat cronch. auto.
+        - inv H2. unfold concretize in H4. rewrite H4.
+          destruct ty1; try congruence; repeat cronch; simpl; auto.
+        - inv H2. unfold concretize in H0. rewrite H0.
+          repeat cronch; simpl; auto.
+        - destruct (is_val_list el) eqn:?.
+          + unfold Genv.find_funct in H. rewrite H. rewrite H1. rewrite H0. cronch.
+            eapply sem_cast_arguments_complete in H2. destruct H2 as [vtl [res [A [B C]]]].
+            repeat chomp. rewrite B. rewrite C. simpl. eauto.
+          + eapply sem_cast_arguments_complete in H2. repeat doinv. repeat chomp. discriminate.
+        - destruct (is_val_list el) eqn:?.
+          + eapply sem_cast_arguments_complete in H. destruct H as [vtl [res [A [B C]]]].
+            repeat chomp. rewrite B. rewrite C. simpl. eauto.
+          + eapply sem_cast_arguments_complete in H. repeat doinv. repeat chomp. discriminate.
+      Qed.
+      
+      Lemma callred_topred:
+        forall lc ps pct pct' a fd fpt args ty te m ps',
+          callred ge lc pct a m fd fpt args ty pct' ps ps' ->
+          exists rule, step_expr ge ce e w RV lc ps pct a te m = topred (Callred rule fd fpt args ty te m pct' ps').
+      Proof.
+        induction 1; cbn.
+        - exploit sem_cast_arguments_complete; eauto. intros [vtl [res [A [B RES]]]].
+          unfold find_funct in H.
+          rewrite A; rewrite H; rewrite H1; rewrite H0; rewrite dec_eq_true; rewrite B; rewrite RES.
+          simpl. eauto.
+        - exploit sem_cast_arguments_complete; eauto. intros [vtl [res [A [B RES]]]].
+          rewrite A; rewrite B; rewrite RES. simpl. eauto.  
+      Qed.
+
+      Definition reducts_incl {A B: Type} (C: A -> B) (res1: reducts A) (res2: reducts B) : Prop :=
+        forall C1 rd, In (C1, rd) res1 -> In ((fun x => C(C1 x)), rd) res2.
+
+      Lemma reducts_incl_trans:
+        forall (A1 A2: Type) (C: A1 -> A2) res1 res2, reducts_incl C res1 res2 ->
+                                                      forall (A3: Type) (C': A2 -> A3) res3,
+                                                        reducts_incl C' res2 res3 ->
+                                                        reducts_incl (fun x => C'(C x)) res1 res3.
+      Proof.
+        unfold reducts_incl; intros. auto.
+      Qed.
+
+      Lemma reducts_incl_nil:
+        forall (A B: Type) (C: A -> B) res,
+          reducts_incl C nil res.
+      Proof.
+        intros; red. intros; contradiction.
+      Qed.
+
+      Lemma reducts_incl_val:
+        forall (A: Type) lc ps pct a te m v ty (C: expr -> A) res,
+          is_val a = Some(v, ty) -> reducts_incl C (step_expr ge ce e w RV lc ps pct a te m) res.
+      Proof.
+        intros. rewrite (is_val_inv _ _ _ H). apply reducts_incl_nil.
+      Qed.
+
+      Lemma reducts_incl_loc:
+        forall (A: Type) lc ps pct a te m l ty (C: expr -> A) res,
+          is_loc a = Some(l, ty) -> reducts_incl C (step_expr ge ce e w LV lc ps pct a te m) res.
+      Proof.
+        intros. rewrite (is_loc_inv _ _ _ H). apply reducts_incl_nil.
+      Qed.
+
+      Lemma reducts_incl_listval:
+        forall (A: Type) lc ps pct a te m vtl (C: exprlist -> A) res,
+          is_val_list a = Some vtl -> reducts_incl C (step_exprlist ge ce e w lc ps pct a te m) res.
+      Proof.
+        intros. rewrite step_exprlist_val_list. apply reducts_incl_nil. congruence.
+      Qed.
+
+      Lemma reducts_incl_incontext:
+        forall (A B: Type) (C: A -> B) res,
+          reducts_incl C res (incontext C res).
+      Proof.
+        unfold reducts_incl, incontext. intros.
+        set (f := fun z : (expr -> A) * reduction => (fun x : expr => C (fst z x), snd z)).
+        change (In (f (C1, rd)) (map f res)). apply in_map. auto.
+      Qed.
+
+      Lemma reducts_incl_incontext2_left:
+        forall (A1 A2 B: Type) (C1: A1 -> B) res1 (C2: A2 -> B) res2,
+          reducts_incl C1 res1 (incontext2 C1 res1 C2 res2).
+      Proof.
+        unfold reducts_incl, incontext2, incontext. intros.
+        rewrite in_app_iff. left.
+        set (f := fun z : (expr -> A1) * reduction => (fun x : expr => C1 (fst z x), snd z)).
+        change (In (f (C0, rd)) (map f res1)). apply in_map; auto.
+      Qed.
+
+      Lemma reducts_incl_incontext2_right:
+        forall (A1 A2 B: Type) (C1: A1 -> B) res1 (C2: A2 -> B) res2,
+          reducts_incl C2 res2 (incontext2 C1 res1 C2 res2).
+      Proof.
+        unfold reducts_incl, incontext2, incontext. intros.
+        rewrite in_app_iff. right.
+        set (f := fun z : (expr -> A2) * reduction => (fun x : expr => C2 (fst z x), snd z)).
+        change (In (f (C0, rd)) (map f res2)). apply in_map; auto.
+      Qed.
+
+      Local Hint Resolve reducts_incl_val reducts_incl_loc reducts_incl_listval
+            reducts_incl_incontext reducts_incl_incontext2_left
+            reducts_incl_incontext2_right : core.
+
+      Lemma step_expr_context:
+        forall from to C,
+          context from to C ->
+          forall lc ps pct a te m,
+            reducts_incl C (step_expr ge ce e w from lc ps pct a te m)
+                         (step_expr ge ce e w to lc ps pct (C a) te m)
+      with step_exprlist_context:
+        forall from C,
+          contextlist from C ->
+          forall lc ps pct a te m,
+            reducts_incl C (step_expr ge ce e w from lc ps pct a te m)
+                         (step_exprlist ge ce e w lc ps pct (C a) te m).
+      Proof.
+        induction 1; cbn; intros.
+        (* top *)
+        - red. destruct (step_expr ge ce e w k lc ps pct a te m); auto.
+        (* deref *)
+        - eapply reducts_incl_trans with (C' := fun x => Ederef x ty); eauto.
+          destruct (is_val (C a)) as [[[v vt] ty']|] eqn:?; eauto.
+        (* field *)
+        - eapply reducts_incl_trans with (C' := fun x => Efield x f ty); eauto.
+          destruct (is_val (C a)) as [[[v vt] ty']|] eqn:?; eauto.
+        (* valof *)
+        - eapply reducts_incl_trans with (C' := fun x => Evalof x ty); eauto.
+          destruct (is_loc (C a)) as [[l ty']|] eqn:?; eauto.
+        (* addrof *)
+        - eapply reducts_incl_trans with (C' := fun x => Eaddrof x ty); eauto.
+          destruct (is_loc (C a)) as [[l ty']|] eqn:?; eauto.
+        (* unop *)
+        - eapply reducts_incl_trans with (C' := fun x => Eunop op x ty); eauto.
+          destruct (is_val (C a)) as [[[v vt] ty']|] eqn:?; eauto.
+        (* binop left *)
+        - eapply reducts_incl_trans with (C' := fun x => Ebinop op x e2 ty); eauto.
+          destruct (is_val (C a)) as [[[v vt] ty']|] eqn:?; eauto.
+        (* binop right *)
+        - eapply reducts_incl_trans with (C' := fun x => Ebinop op e1 x ty); eauto.
+          destruct (is_val e1) as [[[v1 vt1] ty1]|] eqn:?; eauto.
+          destruct (is_val (C a)) as [[[v2 vt2] ty2]|] eqn:?; eauto.
+        (* cast *)
+        - eapply reducts_incl_trans with (C' := fun x => Ecast x ty); eauto.
+          destruct (is_val (C a)) as [[[v vt] ty']|] eqn:?; eauto.
+        (* seqand *)
+        - eapply reducts_incl_trans with (C' := fun x => Eseqand x r2 ty); eauto.
+          destruct (is_val (C a)) as [[[v vt] ty']|] eqn:?; eauto.
+        (* seqor *)
+        - eapply reducts_incl_trans with (C' := fun x => Eseqor x r2 ty); eauto.
+          destruct (is_val (C a)) as [[[v vt] ty']|] eqn:?; eauto.
+        (* condition *)
+        - eapply reducts_incl_trans with (C' := fun x => Econdition x r2 r3 ty); eauto.
+          destruct (is_val (C a)) as [[[v vt] ty']|] eqn:?; eauto.
+        (* assign left *)
+        - eapply reducts_incl_trans with (C' := fun x => Eassign x e2 ty); eauto.
+          destruct (is_loc (C a)) as [[l ty']|] eqn:?; eauto.
+        (* assign right *)
+        - eapply reducts_incl_trans with (C' := fun x => Eassign e1 x ty); eauto.
+          destruct (is_loc e1) as [[[ofs pt bf|b|b pt|ef pt] ty1]|] eqn:?; eauto;
+            destruct (is_val (C a)) as [[[v2 vt2] ty2]|] eqn:?; eauto.
+        (* assignop left *)
+        - eapply reducts_incl_trans with (C' := fun x => Eassignop op x e2 tyres ty); eauto.
+          destruct (is_loc (C a)) as [[l ty']|] eqn:?; eauto.
+        (* assignop right *)
+        - eapply reducts_incl_trans with (C' := fun x => Eassignop op e1 x tyres ty); eauto.
+          destruct (is_loc e1) as [[[ofs pt bf|b|b pt|ef pt] ty1]|] eqn:?; eauto;
+            destruct (is_val (C a)) as [[[v2 vt2] ty2]|] eqn:?; eauto.
+        (* postincr *)
+        - eapply reducts_incl_trans with (C' := fun x => Epostincr id x ty); eauto.
+          destruct (is_loc (C a)) as [[l ty']|] eqn:?; eauto.
+        (* call left *)
+        - eapply reducts_incl_trans with (C' := fun x => Ecall x el ty); eauto.
+          destruct (is_val (C a)) as [[[v vt] ty']|] eqn:?; eauto.
+        (* call right *)
+        - eapply reducts_incl_trans with (C' := fun x => Ecall e1 x ty).
+          apply step_exprlist_context. auto.
+          destruct (is_val e1) as [[[v1 vt1] ty1]|] eqn:?; eauto.
+          destruct (is_val_list (C a)) as [vl|] eqn:?; eauto.
+          destruct v1 eqn:?; eauto.
+        (* comma *)
+        - eapply reducts_incl_trans with (C' := fun x => Ecomma x e2 ty); eauto.
+          destruct (is_val (C a)) as [[[v vt] ty']|] eqn:?; eauto.
+        (* paren *)
+        - eapply reducts_incl_trans with (C' := fun x => Eparen x tycast ty); eauto.
+          destruct (is_val (C a)) as [[[v vt] ty']|] eqn:?; eauto.
+          
+        - induction 1; cbn; intros.
+          (* cons left *)
+          + eapply reducts_incl_trans with (C' := fun x => Econs x el).
+            apply step_expr_context; eauto. eauto.
+          (* binop right *)
+          + eapply reducts_incl_trans with (C' := fun x => Econs e1 x).
+            apply step_exprlist_context; eauto. eauto.
+      Qed.
+
+      (** Completeness part 2: if we can reduce to [Stuckstate], [step_expr]
+          contains at least one [Stuckred] reduction. *)
+
+      Lemma not_stuckred_imm_safe:
+        forall lc te m a k ps pct,
+          (forall C, ~(In (C, Stuckred) (step_expr ge ce e w k lc ps pct a te m))) ->
+          imm_safe_t ge ce e w k lc a ps pct te m.
+      Proof.
+        intros. generalize (step_expr_sound lc ps pct a k te m). intros [A B].
+        destruct (step_expr ge ce e w k lc ps pct a te m) as [|[C rd] res] eqn:?.
+        specialize (B (eq_refl _)). destruct k.
+        destruct a; simpl in B; try congruence. constructor.
+        destruct a; simpl in B; try congruence. constructor.
+        assert (NOTSTUCK: (rd <> Stuckred)).
+        { red; intros. elim (H C). subst rd; auto with coqlib. }
+        exploit A. eauto with coqlib. intros [a' [k' [P [Q R]]]].
+        destruct k'; destruct rd; simpl in R; intuition; try (exfalso; eapply NOTSTUCK; auto; fail).
+        - subst a. eapply imm_safe_t_lred; eauto. 
+        - subst a. eapply imm_safe_t_lfailred; eauto.
+        - subst a. destruct H1 as [w' PT]. eapply imm_safe_t_rred; eauto.
+        - subst. eapply imm_safe_t_callred; eauto.
+        - subst. destruct H1 as [w' PT]. eapply imm_safe_t_rfailred; eauto.
+      Qed.
+      
+      Lemma not_imm_safe_stuck_red:
+        forall lc te m ps pct a k C,
+          context k RV C ->
+          ~imm_safe_t ge ce e w k lc a ps pct te m ->
+          exists C', In (C', Stuckred) (step_expr ge ce e w RV lc ps pct (C a) te m).
+      Proof.
+        intros.
+        assert (exists C', In (C', Stuckred) (step_expr ge ce e w k lc ps pct a te m)).
+        { destruct (classic (exists C', In (C', Stuckred) (step_expr ge ce e w k lc ps pct a te m))); auto.
+          elim H0. apply not_stuckred_imm_safe. apply not_ex_all_not. auto. }
+        destruct H1 as [C' IN].
+        specialize (step_expr_context _ _ _ H lc ps pct a te m). unfold reducts_incl.
+        intro.
+        exists (fun x => (C (C' x))). apply H1; auto.
+      Qed.
+
+    End EXPRS.
+    End EXEC.
+  End Inner.
+End ExprProof.
